theories/opsem.v
@@ -21,48 +21,60 @@ Variable host_instance : host.
 Let store_record := store_record host_function.
 Let host_state := host_state host_instance.
 
+
+
 Inductive reduce_simple : seq administrative_instruction -> seq administrative_instruction -> Prop :=
 
 (** unop **)
 | rs_unop : forall v op t,
-    reduce_simple [::$VA v; AI_basic (BI_unop t op)] [::$VA (@app_unop op v)]
+    reduce_simple [::$VAN v; AI_basic (BI_unop t op)] [::$VAN (@app_unop op v)]
                   
 (** binop **)
 | rs_binop_success : forall v1 v2 v op t,
     app_binop op v1 v2 = Some v ->
-    reduce_simple [::$VA v1; $VA v2; AI_basic (BI_binop t op)] [::$VA v]
+    reduce_simple [::$VAN v1; $VAN v2; AI_basic (BI_binop t op)] [::$VAN v]
 | rs_binop_failure : forall v1 v2 op t,
     app_binop op v1 v2 = None ->
-    reduce_simple [::$VA v1; $VA v2; AI_basic (BI_binop t op)] [::AI_trap]
+    reduce_simple [::$VAN v1; $VAN v2; AI_basic (BI_binop t op)] [::AI_trap]
                   
 (** testops **)
 | rs_testop_i32 :
   forall c testop,
-    reduce_simple [::$VA (VAL_int32 c); AI_basic (BI_testop T_i32 testop)] [::$VA (VAL_int32 (wasm_bool (@app_testop_i i32t testop c)))]
+    reduce_simple [::$VAN (VAL_int32 c); AI_basic (BI_testop T_i32 testop)] [::$VAN (VAL_int32 (wasm_bool (@app_testop_i i32t testop c)))]
 | rs_testop_i64 :
   forall c testop,
-    reduce_simple [::$VA (VAL_int64 c); AI_basic (BI_testop T_i64 testop)] [::$VA (VAL_int32 (wasm_bool (@app_testop_i i64t testop c)))]
+    reduce_simple [::$VAN (VAL_int64 c); AI_basic (BI_testop T_i64 testop)] [::$VAN (VAL_int32 (wasm_bool (@app_testop_i i64t testop c)))]
 
 (** relops **)
 | rs_relop: forall v1 v2 t op,
-    reduce_simple [::$VA v1; $VA v2; AI_basic (BI_relop t op)] [::$VA (VAL_int32 (wasm_bool (app_relop op v1 v2)))]
+    reduce_simple [::$VAN v1; $VAN v2; AI_basic (BI_relop t op)] [::$VAN (VAL_int32 (wasm_bool (app_relop op v1 v2)))]
                   
 (** convert and reinterpret **)
 | rs_convert_success :
   forall t1 t2 v v' sx,
     types_agree (T_num t1) (VAL_num v) ->
     cvt t2 sx v = Some v' ->
-    reduce_simple [::$VA v; AI_basic (BI_cvtop t2 CVO_convert t1 sx)] [::$VA v']
+    reduce_simple [::$VAN v; AI_basic (BI_cvtop t2 CVO_convert t1 sx)] [::$VAN v']
 | rs_convert_failure :
   forall t1 t2 v sx,
     types_agree (T_num t1) (VAL_num v) ->
     cvt t2 sx v = None ->
-    reduce_simple [::$VA v; AI_basic (BI_cvtop t2 CVO_convert t1 sx)] [::AI_trap]
+    reduce_simple [::$VAN v; AI_basic (BI_cvtop t2 CVO_convert t1 sx)] [::AI_trap]
 | rs_reinterpret :
   forall t1 t2 v,
     types_agree (T_num t1) (VAL_num v) ->
-    reduce_simple [::$VA v; AI_basic (BI_cvtop t2 CVO_reinterpret t1 None)] [::$VA (wasm_deserialise (bits v) t2)]
+    reduce_simple [::$VAN v; AI_basic (BI_cvtop t2 CVO_reinterpret t1 None)] [::$VAN (wasm_deserialise (bits v) t2)]
 
+(** reference operations **)
+| rs_ref_is_null_true:
+  forall t,
+    reduce_simple [:: AI_basic (BI_ref_null t); AI_basic BI_ref_is_null] [::$VAN (VAL_int32 Wasm_int.Int32.one)]
+(* This formulation might cause some difficulty in the proofs, but it's the most faithful
+to the spec *)
+| rs_ref_is_null_false:
+  forall ref,
+    (forall t, ref <> VAL_ref_null t) ->
+    reduce_simple [:: v_to_e (VAL_ref ref); AI_basic BI_ref_is_null] [::$VAN (VAL_int32 Wasm_int.Int32.one)]
 (** control-flow operations **)
 | rs_unreachable :
   reduce_simple [::AI_basic BI_unreachable] [::AI_trap]
@@ -70,15 +82,15 @@ Inductive reduce_simple : seq administrative_instruction -> seq administrative_i
   reduce_simple [::AI_basic BI_nop] [::]
 | rs_drop :
   forall v,
-    reduce_simple [::$VA v; AI_basic BI_drop] [::]
+    reduce_simple [::$VAN v; AI_basic BI_drop] [::]
 | rs_select_false :
   forall n v1 v2 ot,
     n = Wasm_int.int_zero i32m ->
-    reduce_simple [::$VA v1; $VA v2; $VA (VAL_int32 n); AI_basic (BI_select ot)] [::$VA v2]
+    reduce_simple [::$VAN v1; $VAN v2; $VAN (VAL_int32 n); AI_basic (BI_select ot)] [::$VAN v2]
 | rs_select_true :
   forall n v1 v2 ot,
     n <> Wasm_int.int_zero i32m ->
-    reduce_simple [::$VA v1; $VA v2; $VA (VAL_int32 n); AI_basic (BI_select ot)] [::$VA v1]
+    reduce_simple [::$VAN v1; $VAN v2; $VAN (VAL_int32 n); AI_basic (BI_select ot)] [::$VAN v1]
 | rs_label_const :
   forall n es vs,
     const_list vs ->
@@ -95,20 +107,20 @@ Inductive reduce_simple : seq administrative_instruction -> seq administrative_i
 | rs_br_if_false :
   forall n i,
     n = Wasm_int.int_zero i32m ->
-    reduce_simple [::$VA (VAL_int32 n); AI_basic (BI_br_if i)] [::]
+    reduce_simple [::$VAN (VAL_int32 n); AI_basic (BI_br_if i)] [::]
 | rs_br_if_true :
   forall n i,
     n <> Wasm_int.int_zero i32m ->
-    reduce_simple [::$VA (VAL_int32 n); AI_basic (BI_br_if i)] [::AI_basic (BI_br i)]
+    reduce_simple [::$VAN (VAL_int32 n); AI_basic (BI_br_if i)] [::AI_basic (BI_br i)]
 | rs_br_table :
   forall iss c i j,
     length iss > Wasm_int.nat_of_uint i32m c ->
     List.nth_error iss (Wasm_int.nat_of_uint i32m c) = Some j ->
-    reduce_simple [::$VA (VAL_int32 c); AI_basic (BI_br_table iss i)] [::AI_basic (BI_br j)]
+    reduce_simple [::$VAN (VAL_int32 c); AI_basic (BI_br_table iss i)] [::AI_basic (BI_br j)]
 | rs_br_table_length :
   forall iss c i,
     length iss <= (Wasm_int.nat_of_uint i32m c) ->
-    reduce_simple [::$VA (VAL_int32 c); AI_basic (BI_br_table iss i)] [::AI_basic (BI_br i)]
+    reduce_simple [::$VAN (VAL_int32 c); AI_basic (BI_br_table iss i)] [::AI_basic (BI_br i)]
 | rs_local_const :
   forall es n f,
     const_list es ->
@@ -137,9 +149,13 @@ Inductive reduce_simple : seq administrative_instruction -> seq administrative_i
 Inductive reduce : host_state -> store_record -> frame -> list administrative_instruction ->
                    host_state -> store_record -> frame -> list administrative_instruction -> Prop :=
 | r_simple :
-  forall e e' s f hs,
+  forall hs s f e e',
     reduce_simple e e' ->
     reduce hs s f e hs s f e'
+| r_ref_func:
+  forall hs s f addr x,
+    lookup_N f.(f_inst).(inst_funcs) x = Some addr ->
+    reduce hs s f [::AI_basic (BI_ref_func x)] hs s f [::AI_ref addr]
 | r_block :
   forall hs s f vs es n m tb t1s t2s,
     expand f.(f_inst) tb = Some (Tf t1s t2s) ->
@@ -164,7 +180,7 @@ Inductive reduce : host_state -> store_record -> frame -> list administrative_in
     length vs = m ->
     length t1s = m ->
     length t2s = n ->
-    reduce hs s f (vs ++ [::$VA (VAL_int32 c); AI_basic (BI_if tb es1 es2)]) hs s f [::AI_label n [::] (vs ++ to_e_list es2)]
+    reduce hs s f (vs ++ [::$VAN (VAL_int32 c); AI_basic (BI_if tb es1 es2)]) hs s f [::AI_label n [::] (vs ++ to_e_list es2)]
 | rs_if_true :
   forall hs s f c vs es1 es2 n m tb t1s t2s,
     expand f.(f_inst) tb = Some (Tf t1s t2s) ->
@@ -173,7 +189,7 @@ Inductive reduce : host_state -> store_record -> frame -> list administrative_in
     length vs = m ->
     length t1s = m ->
     length t2s = n ->
-    reduce hs s f (vs ++ [::$VA (VAL_int32 c); AI_basic (BI_if tb es1 es2)]) hs s f [::AI_label n [::] (vs ++ to_e_list es1)]
+    reduce hs s f (vs ++ [::$VAN (VAL_int32 c); AI_basic (BI_if tb es1 es2)]) hs s f [::AI_label n [::] (vs ++ to_e_list es1)]
 (** calling operations **)
 | r_call :
   forall s f (i: funcidx) a hs,
@@ -184,26 +200,26 @@ Inductive reduce : host_state -> store_record -> frame -> list administrative_in
     stab_elem s f.(f_inst) x (Wasm_int.nat_of_uint i32m i) = Some (VAL_ref_func a) ->
     List.nth_error s.(s_funcs) (N.to_nat a) = Some cl ->
     List.nth_error f.(f_inst).(inst_types) (N.to_nat y) = Some (cl_type cl) ->
-    reduce hs s f [::$VA (VAL_int32 i); AI_basic (BI_call_indirect x y)] hs s f [::AI_invoke a]
+    reduce hs s f [::$VAN (VAL_int32 i); AI_basic (BI_call_indirect x y)] hs s f [::AI_invoke a]
 | r_call_indirect_failure1 :
   forall s f x (y: typeidx) a cl i hs,
     stab_elem s f.(f_inst) x (Wasm_int.nat_of_uint i32m i) = Some (VAL_ref_func a) ->
     List.nth_error s.(s_funcs) (N.to_nat a) = Some cl ->
     List.nth_error f.(f_inst).(inst_types) (N.to_nat y) <> Some (cl_type cl) ->
-    reduce hs s f [::$VA (VAL_int32 i); AI_basic (BI_call_indirect x y)] hs s f [::AI_trap]
+    reduce hs s f [::$VAN (VAL_int32 i); AI_basic (BI_call_indirect x y)] hs s f [::AI_trap]
 | r_call_indirect_failure2 :
   forall s f x (y: typeidx) a i hs,
     stab_elem s f.(f_inst) x (Wasm_int.nat_of_uint i32m i) = Some (VAL_ref_func a) ->
     List.nth_error s.(s_funcs) (N.to_nat a) = None ->
-    reduce hs s f [::$VA (VAL_int32 i); AI_basic (BI_call_indirect x y)] hs s f [::AI_trap]
+    reduce hs s f [::$VAN (VAL_int32 i); AI_basic (BI_call_indirect x y)] hs s f [::AI_trap]
 | r_call_indirect_failure3 :
   forall s f x (y: typeidx) i hs,
     stab_elem s f.(f_inst) x (Wasm_int.nat_of_uint i32m i) = None ->
-    reduce hs s f [::$VA (VAL_int32 i); AI_basic (BI_call_indirect x y)] hs s f [::AI_trap]
+    reduce hs s f [::$VAN (VAL_int32 i); AI_basic (BI_call_indirect x y)] hs s f [::AI_trap]
 | r_call_indirect_failure4 :
   forall s f x (y: typeidx) i hs t,
     stab_elem s f.(f_inst) x (Wasm_int.nat_of_uint i32m i) = Some (VAL_ref_null t) ->
-    reduce hs s f [::$VA (VAL_int32 i); AI_basic (BI_call_indirect x y)] hs s f [::AI_trap]
+    reduce hs s f [::$VAN (VAL_int32 i); AI_basic (BI_call_indirect x y)] hs s f [::AI_trap]
 | r_invoke_native :
   forall a cl t1s t2s ts es ves vcs n m k zs s f f' i hs,
     List.nth_error s.(s_funcs) (N.to_nat a) = Some cl ->
@@ -219,7 +235,7 @@ Inductive reduce : host_state -> store_record -> frame -> list administrative_in
     reduce hs s f (ves ++ [::AI_invoke a]) hs s f [::AI_local m f' [::AI_label m [::] (to_e_list es)]]
 | r_invoke_host_success :
   forall a cl h t1s t2s ves vcs m n s s' r f hs hs',
-    List.nth_error s.(s_funcs) (N.to_nat a) = Some cl ->
+    lookup_N s.(s_funcs) a = Some cl ->
     cl = FC_func_host (Tf t1s t2s) h ->
     ves = v_to_e_list vcs ->
     length vcs = n ->
@@ -229,7 +245,7 @@ Inductive reduce : host_state -> store_record -> frame -> list administrative_in
     reduce hs s f (ves ++ [::AI_invoke a]) hs' s' f (result_to_stack r)
 | r_invoke_host_diverge :
   forall a cl t1s t2s h ves vcs n m s f hs hs',
-    List.nth_error s.(s_funcs) (N.to_nat a) = Some cl ->
+    lookup_N s.(s_funcs) a = Some cl ->
     cl = FC_func_host (Tf t1s t2s) h ->
     ves = v_to_e_list vcs ->
     length vcs = n ->
@@ -241,70 +257,70 @@ Inductive reduce : host_state -> store_record -> frame -> list administrative_in
 (** get, set, load, and store operations **)
 | r_local_get :
   forall f v j s hs,
-    List.nth_error f.(f_locs) (N.to_nat j) = Some v ->
-    reduce hs s f [::AI_basic (BI_local_get j)] hs s f [::AI_basic (BI_const v)]
+    lookup_N f.(f_locs) j = Some v ->
+    reduce hs s f [::AI_basic (BI_local_get j)] hs s f [::v_to_e v]
 | r_local_set :
   forall f f' i v s vd hs,
     f'.(f_inst) = f.(f_inst) ->
     N.to_nat i < length f.(f_locs) ->
     f'.(f_locs) = set_nth vd f.(f_locs) (N.to_nat i) v ->
-    reduce hs s f [::AI_basic (BI_const v); AI_basic (BI_local_set i)] hs s f' [::]
+    reduce hs s f [::v_to_e v; AI_basic (BI_local_set i)] hs s f' [::]
 | r_global_get :
   forall s f i v hs,
     sglob_val s f.(f_inst) (N.to_nat i) = Some v ->
-    reduce hs s f [::AI_basic (BI_global_get i)] hs s f [::AI_basic (BI_const v)]
+    reduce hs s f [::AI_basic (BI_global_get i)] hs s f [::v_to_e v]
 | r_global_set :
   forall s f i v s' hs,
     supdate_glob s f.(f_inst) (N.to_nat i) v = Some s' ->
-    reduce hs s f [::AI_basic (BI_const v); AI_basic (BI_global_set i)] hs s' f [::]
+    reduce hs s f [::v_to_e v; AI_basic (BI_global_set i)] hs s' f [::]
            
 (** table **)
 | r_table_get_success :
   forall x i tabv s f hs,
-    stab_elem s f.(f_inst) x (Wasm_int.nat_of_uint i32m i) = Some tabv ->
-    reduce hs s f [::$VA (VAL_int32 i); AI_basic (BI_table_get x)] hs s f [::AI_basic (BI_const (VAL_ref tabv))]
+    stab_elem s f.(f_inst) x (Wasm_int.N_of_uint i32m i) = Some tabv ->
+    reduce hs s f [::$VAN (VAL_int32 i); AI_basic (BI_table_get x)] hs s f [::v_to_e (VAL_ref tabv)]
 | r_table_get_failure :
   forall x i s f hs,
-    stab_elem s f.(f_inst) x (Wasm_int.nat_of_uint i32m i) = None ->
-    reduce hs s f [::$VA (VAL_int32 i); AI_basic (BI_table_get x)] hs s f [::AI_trap]
+    stab_elem s f.(f_inst) x (Wasm_int.N_of_uint i32m i) = None ->
+    reduce hs s f [::$VAN (VAL_int32 i); AI_basic (BI_table_get x)] hs s f [::AI_trap]
 | r_table_set_success :
   forall x i tabv s s' f hs,
-    stab_update s f.(f_inst) x (Wasm_int.nat_of_uint i32m i) tabv = Some s' ->
-    reduce hs s f [::$VA (VAL_int32 i); AI_basic (BI_const (VAL_ref tabv)); AI_basic (BI_table_set x)] hs s' f [::]
+    stab_update s f.(f_inst) x (Wasm_int.N_of_uint i32m i) tabv = Some s' ->
+    reduce hs s f [::$VAN (VAL_int32 i); v_to_e (VAL_ref tabv); AI_basic (BI_table_set x)] hs s' f [::]
 | r_table_set_failure :
   forall x i tabv s s' f hs,
-    stab_update s f.(f_inst) x (Wasm_int.nat_of_uint i32m i) tabv = None ->
-    reduce hs s f [::$VA (VAL_int32 i); AI_basic (BI_const (VAL_ref tabv)); AI_basic (BI_table_set x)] hs s' f [::]
+    stab_update s f.(f_inst) x (Wasm_int.N_of_uint i32m i) tabv = None ->
+    reduce hs s f [::$VAN (VAL_int32 i); v_to_e (VAL_ref tabv); AI_basic (BI_table_set x)] hs s' f [::]
 | r_table_size :
   forall x tab sz s s' f hs,
     stab s f.(f_inst) x = Some tab ->
     tab_size tab = sz ->
-    reduce hs s f [:: AI_basic (BI_table_size x)] hs s' f [::$VA (VAL_int32 (Wasm_int.int_of_Z i32m (Z.of_nat sz)))]
+    reduce hs s f [:: AI_basic (BI_table_size x)] hs s' f [::$VAN (VAL_int32 (Wasm_int.int_of_Z i32m (Z.of_nat sz)))]
 | r_table_grow_success :
   forall x n tab sz tabinit s s' f hs,
     stab s f.(f_inst) x = Some tab ->
     tab_size tab = sz ->
     stab_grow s f.(f_inst) x (Wasm_int.N_of_uint i32m n) tabinit = Some s' ->
-    reduce hs s f [::AI_basic (BI_const (VAL_ref tabinit)); $VA (VAL_int32 n); AI_basic (BI_table_set x)]
-      hs s' f [::$VA (VAL_int32 (Wasm_int.int_of_Z i32m (Z.of_nat sz)))]
+    reduce hs s f [::v_to_e (VAL_ref tabinit); $VAN (VAL_int32 n); AI_basic (BI_table_set x)]
+      hs s' f [::$VAN (VAL_int32 (Wasm_int.int_of_Z i32m (Z.of_nat sz)))]
 | r_table_grow_failure :
   forall x n tab sz tabinit s s' f hs,
     stab s f.(f_inst) x = Some tab ->
     tab_size tab = sz ->
-    reduce hs s f [::AI_basic (BI_const (VAL_ref tabinit)); $VA (VAL_int32 n); AI_basic (BI_table_set x)]
-      hs s' f [::$VA (VAL_int32 int32_minus_one)]
+    reduce hs s f [::v_to_e (VAL_ref tabinit); $VAN (VAL_int32 n); AI_basic (BI_table_set x)]
+      hs s' f [::$VAN (VAL_int32 int32_minus_one)]
 | r_table_fill_bound :
   forall x i n tab tabv s s' f hs,
     stab s f.(f_inst) x = Some tab ->
     (Wasm_int.N_of_uint i32m i) + (Wasm_int.N_of_uint i32m n) > tab_size tab ->
-    reduce hs s f [::$VA (VAL_int32 i); AI_basic (BI_const (VAL_ref tabv)); $VA (VAL_int32 n); AI_basic (BI_table_fill x)]
+    reduce hs s f [::$VAN (VAL_int32 i); v_to_e (VAL_ref tabv); $VAN (VAL_int32 n); AI_basic (BI_table_fill x)]
       hs s' f [::AI_trap]
 | r_table_fill_return :
   forall x i n tab tabv s f hs,
     stab s f.(f_inst) x = Some tab ->
     (Wasm_int.N_of_uint i32m i) + (Wasm_int.N_of_uint i32m n) <= tab_size tab ->
     n = Wasm_int.int_zero i32m ->
-    reduce hs s f [::$VA (VAL_int32 i); AI_basic (BI_const (VAL_ref tabv)); $VA (VAL_int32 n); AI_basic (BI_table_fill x)]
+    reduce hs s f [::$VAN (VAL_int32 i); v_to_e (VAL_ref tabv); $VAN (VAL_int32 n); AI_basic (BI_table_fill x)]
       hs s f [::]
 | r_table_fill_step :
   forall x i n tab tabv n' i' s f hs,
@@ -313,16 +329,16 @@ Inductive reduce : host_state -> store_record -> frame -> list administrative_in
     n <> Wasm_int.int_zero i32m ->
     Wasm_int.N_of_uint i32m n' = N.sub (Wasm_int.N_of_uint i32m n) 1 ->
     Wasm_int.N_of_uint i32m i' = N.add (Wasm_int.N_of_uint i32m i) 1 ->
-    reduce hs s f [::$VA (VAL_int32 i); AI_basic (BI_const (VAL_ref tabv)); $VA (VAL_int32 n); AI_basic (BI_table_fill x)]
-      hs s f [::$VA (VAL_int32 i); AI_basic (BI_const (VAL_ref tabv)); AI_basic (BI_table_set x);
-              $VA (VAL_int32 i'); AI_basic (BI_const (VAL_ref tabv)); $VA (VAL_int32 n'); AI_basic (BI_table_fill x)]
+    reduce hs s f [::$VAN (VAL_int32 i); v_to_e (VAL_ref tabv); $VAN (VAL_int32 n); AI_basic (BI_table_fill x)]
+      hs s f [::$VAN (VAL_int32 i); v_to_e (VAL_ref tabv); AI_basic (BI_table_set x);
+              $VAN (VAL_int32 i'); v_to_e (VAL_ref tabv); $VAN (VAL_int32 n'); AI_basic (BI_table_fill x)]
 | r_table_copy_bound :
   forall x y src dst n tabx taby s f hs,
     stab s f.(f_inst) x = Some tabx ->
     stab s f.(f_inst) y = Some taby ->
     (((Wasm_int.N_of_uint i32m src) + (Wasm_int.N_of_uint i32m n) > tab_size taby) \/
        ((Wasm_int.N_of_uint i32m dst) + (Wasm_int.N_of_uint i32m n) > tab_size tabx)) ->
-    reduce hs s f [::$VA (VAL_int32 dst); $VA (VAL_int32 src); $VA (VAL_int32 n); AI_basic (BI_table_copy x y)]
+    reduce hs s f [::$VAN (VAL_int32 dst); $VAN (VAL_int32 src); $VAN (VAL_int32 n); AI_basic (BI_table_copy x y)]
       hs s f [::AI_trap]
 | r_table_copy_return :
   forall x y src dst n tabx taby s f hs,
@@ -331,7 +347,7 @@ Inductive reduce : host_state -> store_record -> frame -> list administrative_in
     ((Wasm_int.N_of_uint i32m src) + (Wasm_int.N_of_uint i32m n) <= tab_size taby) ->
     ((Wasm_int.N_of_uint i32m dst) + (Wasm_int.N_of_uint i32m n) <= tab_size tabx) ->
     n = Wasm_int.int_zero i32m ->
-    reduce hs s f [::$VA (VAL_int32 dst); $VA (VAL_int32 src); $VA (VAL_int32 n); AI_basic (BI_table_copy x y)]
+    reduce hs s f [::$VAN (VAL_int32 dst); $VAN (VAL_int32 src); $VAN (VAL_int32 n); AI_basic (BI_table_copy x y)]
       hs s f [::]
 | r_table_copy_forward :
   forall x y src dst n tabx taby src' dst' n' s f hs,
@@ -344,9 +360,9 @@ Inductive reduce : host_state -> store_record -> frame -> list administrative_in
     Wasm_int.N_of_uint i32m n' = N.sub (Wasm_int.N_of_uint i32m n) 1 ->
     Wasm_int.N_of_uint i32m src' = N.add (Wasm_int.N_of_uint i32m src) 1 ->
     Wasm_int.N_of_uint i32m dst' = N.add (Wasm_int.N_of_uint i32m dst) 1 ->
-    reduce hs s f [::$VA (VAL_int32 dst); $VA (VAL_int32 src); $VA (VAL_int32 n); AI_basic (BI_table_copy x y)]
-      hs s f [:: $VA (VAL_int32 dst); $VA (VAL_int32 src); AI_basic (BI_table_get y); AI_basic (BI_table_get x);
-              $VA (VAL_int32 dst'); $VA (VAL_int32 src'); $VA (VAL_int32 n'); AI_basic (BI_table_copy x y)]
+    reduce hs s f [::$VAN (VAL_int32 dst); $VAN (VAL_int32 src); $VAN (VAL_int32 n); AI_basic (BI_table_copy x y)]
+      hs s f [:: $VAN (VAL_int32 dst); $VAN (VAL_int32 src); AI_basic (BI_table_get y); AI_basic (BI_table_get x);
+              $VAN (VAL_int32 dst'); $VAN (VAL_int32 src'); $VAN (VAL_int32 n'); AI_basic (BI_table_copy x y)]
 | r_table_copy_backward :
   forall x y src dst n tabx taby src' dst' n' s f hs,
     stab s f.(f_inst) x = Some tabx ->
@@ -358,16 +374,16 @@ Inductive reduce : host_state -> store_record -> frame -> list administrative_in
     Wasm_int.N_of_uint i32m n' = N.add (Wasm_int.N_of_uint i32m n) 1 ->
     Wasm_int.N_of_uint i32m src' = N.sub (Wasm_int.N_of_uint i32m src + Wasm_int.N_of_uint i32m n) 1 ->
     Wasm_int.N_of_uint i32m dst' = N.sub (Wasm_int.N_of_uint i32m dst + Wasm_int.N_of_uint i32m n) 1 ->
-    reduce hs s f [::$VA (VAL_int32 dst); $VA (VAL_int32 src); $VA (VAL_int32 n); AI_basic (BI_table_copy x y)]
-      hs s f [:: $VA (VAL_int32 dst'); $VA (VAL_int32 src'); AI_basic (BI_table_get y); AI_basic (BI_table_get x);
-              $VA (VAL_int32 dst); $VA (VAL_int32 src); $VA (VAL_int32 n'); AI_basic (BI_table_copy x y)]
+    reduce hs s f [::$VAN (VAL_int32 dst); $VAN (VAL_int32 src); $VAN (VAL_int32 n); AI_basic (BI_table_copy x y)]
+      hs s f [:: $VAN (VAL_int32 dst'); $VAN (VAL_int32 src'); AI_basic (BI_table_get y); AI_basic (BI_table_get x);
+              $VAN (VAL_int32 dst); $VAN (VAL_int32 src); $VAN (VAL_int32 n'); AI_basic (BI_table_copy x y)]
 | r_table_init_bound :
   forall x y src dst n tab elem s f hs,
     stab s f.(f_inst) x = Some tab ->
     selem s f.(f_inst) y = Some elem ->
     (((Wasm_int.N_of_uint i32m src) + (Wasm_int.N_of_uint i32m n) > elem_size elem) \/
        ((Wasm_int.N_of_uint i32m dst) + (Wasm_int.N_of_uint i32m n) > tab_size tab)) ->
-    reduce hs s f [::$VA (VAL_int32 dst); $VA (VAL_int32 src); $VA (VAL_int32 n); AI_basic (BI_table_init x y)]
+    reduce hs s f [::$VAN (VAL_int32 dst); $VAN (VAL_int32 src); $VAN (VAL_int32 n); AI_basic (BI_table_init x y)]
       hs s f [::AI_trap]
 | r_table_init_return :
   forall x y src dst n tab elem s f hs,
@@ -376,7 +392,7 @@ Inductive reduce : host_state -> store_record -> frame -> list administrative_in
     ((Wasm_int.N_of_uint i32m src) + (Wasm_int.N_of_uint i32m n) <= elem_size elem) ->
     ((Wasm_int.N_of_uint i32m dst) + (Wasm_int.N_of_uint i32m n) <= tab_size tab) ->
     n = Wasm_int.int_zero i32m ->
-    reduce hs s f [::$VA (VAL_int32 dst); $VA (VAL_int32 src); $VA (VAL_int32 n); AI_basic (BI_table_init x y)]
+    reduce hs s f [::$VAN (VAL_int32 dst); $VAN (VAL_int32 src); $VAN (VAL_int32 n); AI_basic (BI_table_init x y)]
       hs s f [::]
 | r_table_init_step :
   forall x y src dst n tab elem src' dst' n' v s f hs,
@@ -389,9 +405,9 @@ Inductive reduce : host_state -> store_record -> frame -> list administrative_in
     Wasm_int.N_of_uint i32m n' = N.sub (Wasm_int.N_of_uint i32m n) 1 ->
     Wasm_int.N_of_uint i32m src' = N.add (Wasm_int.N_of_uint i32m src) 1 ->
     Wasm_int.N_of_uint i32m dst' = N.add (Wasm_int.N_of_uint i32m dst) 1 ->
-    reduce hs s f [::$VA (VAL_int32 dst); $VA (VAL_int32 src); $VA (VAL_int32 n); AI_basic (BI_table_init x y)]
-      hs s f [:: $VA (VAL_int32 dst); AI_basic (BI_const (VAL_ref v)); AI_basic (BI_table_set x);
-              $VA (VAL_int32 dst'); $VA (VAL_int32 src'); $VA (VAL_int32 n'); AI_basic (BI_table_init x y)]
+    reduce hs s f [::$VAN (VAL_int32 dst); $VAN (VAL_int32 src); $VAN (VAL_int32 n); AI_basic (BI_table_init x y)]
+      hs s f [:: $VAN (VAL_int32 dst); v_to_e (VAL_ref v); AI_basic (BI_table_set x);
+              $VAN (VAL_int32 dst'); $VAN (VAL_int32 src'); $VAN (VAL_int32 n'); AI_basic (BI_table_init x y)]
 | r_elem_drop:
   forall x hs s f s',
     selem_drop s f.(f_inst) x = Some s' ->
@@ -403,84 +419,84 @@ Inductive reduce : host_state -> store_record -> frame -> list administrative_in
     smem_ind s f.(f_inst) = Some i ->
     List.nth_error s.(s_mems) i = Some m ->
     load m (Wasm_int.N_of_uint i32m k) off (tnum_length t) = Some bs ->
-    reduce hs s f [::$VA (VAL_int32 k); AI_basic (BI_load t None a off)] hs s f [::$VA (wasm_deserialise bs t)]
+    reduce hs s f [::$VAN (VAL_int32 k); AI_basic (BI_load t None a off)] hs s f [::$VAN (wasm_deserialise bs t)]
 | r_load_failure :
   forall s i f t k a off m hs,
     smem_ind s f.(f_inst) = Some i ->
     List.nth_error s.(s_mems) i = Some m ->
     load m (Wasm_int.N_of_uint i32m k) off (tnum_length t) = None ->
-    reduce hs s f [::$VA (VAL_int32 k); AI_basic (BI_load t None a off)] hs s f [::AI_trap]
+    reduce hs s f [::$VAN (VAL_int32 k); AI_basic (BI_load t None a off)] hs s f [::AI_trap]
 | r_load_packed_success :
   forall s i f t tp k a off m bs sx hs,
     smem_ind s f.(f_inst) = Some i ->
     List.nth_error s.(s_mems) i = Some m ->
     load_packed sx m (Wasm_int.N_of_uint i32m k) off (tp_length tp) (tnum_length t) = Some bs ->
-    reduce hs s f [::$VA (VAL_int32 k); AI_basic (BI_load t (Some (tp, sx)) a off)] hs s f [::$VA (wasm_deserialise bs t)]
+    reduce hs s f [::$VAN (VAL_int32 k); AI_basic (BI_load t (Some (tp, sx)) a off)] hs s f [::$VAN (wasm_deserialise bs t)]
 | r_load_packed_failure :
   forall s i f t tp k a off m sx hs,
     smem_ind s f.(f_inst) = Some i ->
     List.nth_error s.(s_mems) i = Some m ->
     load_packed sx m (Wasm_int.N_of_uint i32m k) off (tp_length tp) (tnum_length t) = None ->
-    reduce hs s f [::$VA (VAL_int32 k); AI_basic (BI_load t (Some (tp, sx)) a off)] hs s f [::AI_trap]
+    reduce hs s f [::$VAN (VAL_int32 k); AI_basic (BI_load t (Some (tp, sx)) a off)] hs s f [::AI_trap]
 | r_store_success :
   forall t v s i f mem' k a off m hs,
     typeof_num v = t ->
     smem_ind s f.(f_inst) = Some i ->
     List.nth_error s.(s_mems) i = Some m ->
     store m (Wasm_int.N_of_uint i32m k) off (bits v) (tnum_length t) = Some mem' ->
-    reduce hs s f [::$VA (VAL_int32 k); $VA v; AI_basic (BI_store t None a off)] hs (upd_s_mem s (set_nth mem' s.(s_mems) i mem')) f [::]
+    reduce hs s f [::$VAN (VAL_int32 k); $VAN v; AI_basic (BI_store t None a off)] hs (upd_s_mem s (set_nth mem' s.(s_mems) i mem')) f [::]
 | r_store_failure :
   forall t v s i f m k off a hs,
     typeof_num v = t ->
     smem_ind s f.(f_inst) = Some i ->
     List.nth_error s.(s_mems) i = Some m ->
     store m (Wasm_int.N_of_uint i32m k) off (bits v) (tnum_length t) = None ->
-    reduce hs s f [::$VA (VAL_int32 k); $VA v; AI_basic (BI_store t None a off)] hs s f [::AI_trap]
+    reduce hs s f [::$VAN (VAL_int32 k); $VAN v; AI_basic (BI_store t None a off)] hs s f [::AI_trap]
 | r_store_packed_success :
   forall t v s i f m k off a mem' tp hs,
     typeof_num v = t ->
     smem_ind s f.(f_inst) = Some i ->
     List.nth_error s.(s_mems) i = Some m ->
     store_packed m (Wasm_int.N_of_uint i32m k) off (bits v) (tp_length tp) = Some mem' ->
-    reduce hs s f [::$VA (VAL_int32 k); $VA v; AI_basic (BI_store t (Some tp) a off)] hs (upd_s_mem s (set_nth mem' s.(s_mems) i mem')) f [::]
+    reduce hs s f [::$VAN (VAL_int32 k); $VAN v; AI_basic (BI_store t (Some tp) a off)] hs (upd_s_mem s (set_nth mem' s.(s_mems) i mem')) f [::]
 | r_store_packed_failure :
   forall t v s i f m k off a tp hs,
     typeof_num v = t ->
     smem_ind s f.(f_inst) = Some i ->
     List.nth_error s.(s_mems) i = Some m ->
     store_packed m (Wasm_int.N_of_uint i32m k) off (bits v) (tp_length tp) = None ->
-    reduce hs s f [::$VA (VAL_int32 k); $VA v; AI_basic (BI_store t (Some tp) a off)] hs s f [::AI_trap]
+    reduce hs s f [::$VAN (VAL_int32 k); $VAN v; AI_basic (BI_store t (Some tp) a off)] hs s f [::AI_trap]
 | r_memory_size :
   forall i f m n s hs,
     smem_ind s f.(f_inst) = Some i ->
     List.nth_error s.(s_mems) i = Some m ->
     mem_size m = n ->
-    reduce hs s f [::AI_basic (BI_memory_size)] hs s f [::$VA (VAL_int32 (Wasm_int.int_of_Z i32m (Z.of_nat n)))]
+    reduce hs s f [::AI_basic (BI_memory_size)] hs s f [::$VAN (VAL_int32 (Wasm_int.int_of_Z i32m (Z.of_nat n)))]
 | r_memory_grow_success :
   forall s i f m n mem' c hs,
     smem_ind s f.(f_inst) = Some i ->
     List.nth_error s.(s_mems) i = Some m ->
     mem_size m = n ->
     mem_grow m (Wasm_int.N_of_uint i32m c) = Some mem' ->
-    reduce hs s f [::$VA (VAL_int32 c); AI_basic BI_memory_grow] hs (upd_s_mem s (set_nth mem' s.(s_mems) i mem')) f [::$VA (VAL_int32 (Wasm_int.int_of_Z i32m (Z.of_nat n)))]
+    reduce hs s f [::$VAN (VAL_int32 c); AI_basic BI_memory_grow] hs (upd_s_mem s (set_nth mem' s.(s_mems) i mem')) f [::$VAN (VAL_int32 (Wasm_int.int_of_Z i32m (Z.of_nat n)))]
 | r_memory_grow_failure :
   forall i f m n s c hs,
     smem_ind s f.(f_inst) = Some i ->
     List.nth_error s.(s_mems) i = Some m ->
     mem_size m = n ->
-    reduce hs s f [::$VA (VAL_int32 c); AI_basic BI_memory_grow] hs s f [::$VA (VAL_int32 int32_minus_one)]
+    reduce hs s f [::$VAN (VAL_int32 c); AI_basic BI_memory_grow] hs s f [::$VAN (VAL_int32 int32_minus_one)]
 | r_memory_fill_bound:
   forall s f mem d n v hs,
     smem s f.(f_inst) = Some mem ->
     (Wasm_int.N_of_uint i32m d) + (Wasm_int.N_of_uint i32m n) > mem_size mem ->
-    reduce hs s f [::$VA (VAL_int32 d); AI_basic (BI_const v); $VA (VAL_int32 n); AI_basic (BI_memory_fill)]
+    reduce hs s f [::$VAN (VAL_int32 d); $VAN (VAL_int32 v); $VAN (VAL_int32 n); AI_basic (BI_memory_fill)]
            hs s f [::AI_trap]
 | r_memory_fill_return:
   forall s f mem d n v hs,
     smem s f.(f_inst) = Some mem ->
     (Wasm_int.N_of_uint i32m d) + (Wasm_int.N_of_uint i32m n) <= mem_size mem ->
     n = Wasm_int.int_zero i32m ->
-    reduce hs s f [::$VA (VAL_int32 d); AI_basic (BI_const v); $VA (VAL_int32 n); AI_basic (BI_memory_fill)]
+    reduce hs s f [::$VAN (VAL_int32 d); $VAN (VAL_int32 v); $VAN (VAL_int32 n); AI_basic (BI_memory_fill)]
            hs s f [::]
 | r_memory_fill_step:
   forall s f mem d n d' n' v hs,
@@ -489,9 +505,9 @@ Inductive reduce : host_state -> store_record -> frame -> list administrative_in
     n <> Wasm_int.int_zero i32m ->
     Wasm_int.N_of_uint i32m n' = N.sub (Wasm_int.N_of_uint i32m n) 1 ->
     Wasm_int.N_of_uint i32m d' = N.add (Wasm_int.N_of_uint i32m d) 1 ->
-    reduce hs s f [::$VA (VAL_int32 d); AI_basic (BI_const v); $VA (VAL_int32 n); AI_basic (BI_memory_fill)]
-      hs s f [::$VA (VAL_int32 d); AI_basic (BI_const v); AI_basic (BI_store T_i32 (Some Tp_i8) N0 N0);
-                $VA (VAL_int32 d'); AI_basic (BI_const v); $VA (VAL_int32 n'); AI_basic (BI_memory_fill)]
+    reduce hs s f [::$VAN (VAL_int32 d); $VAN (VAL_int32 v); $VAN (VAL_int32 n); AI_basic (BI_memory_fill)]
+      hs s f [::$VAN (VAL_int32 d); $VAN (VAL_int32 v); AI_basic (BI_store T_i32 (Some Tp_i8) N0 N0);
+                $VAN (VAL_int32 d'); $VAN (VAL_int32 v); $VAN (VAL_int32 n'); AI_basic (BI_memory_fill)]
 
            
 (** label and local **)
