theories/typing.v
@@ -103,7 +103,14 @@ types in a point-wise manner.
 https://www.w3.org/TR/wasm-core-2/valid/instructions.html
  **)
 Inductive be_typing : t_context -> seq basic_instruction -> function_type -> Prop :=
-| bet_const : forall C v, be_typing C [::BI_const v] (Tf [::] [::typeof v])
+| bet_const_num : forall C v, be_typing C [::BI_const_num v] (Tf [::] [::T_num (typeof_num v)])
+| bet_const_vec : forall C v, be_typing C [::BI_const_vec v] (Tf [::] [::T_vec (typeof_vec v)])
+| bet_ref_null: forall C t, be_typing C [::BI_ref_null t] (Tf [::] [::T_ref t])
+| bet_ref_is_null: forall C t, be_typing C [::BI_ref_is_null] (Tf [::T_ref t] [::T_num T_i32])
+| bet_ref_func: forall C t x,
+    lookup_N (tc_func C) x = Some t ->
+    List.In x (tc_ref C) ->
+    be_typing C [::BI_ref_func x] (Tf [::] [::T_ref T_funcref])
 | bet_unop : forall C t op,
     unop_type_agree t op -> be_typing C [::BI_unop t op] (Tf [::T_num t] [::T_num t])
 | bet_binop : forall C t op,
